Implement arraylists.

src/Utils/UnionFind.v
@@ -4,11 +4,15 @@
    while the instantiation with a function implementation should be closed
    under the global context.
 *)
-Require Import Equalities Orders.
+Require Import Equalities Orders ZArith.
 
 Require Int63 PArray.
 
-Module Type ArrayListOps (Idx : EqLtLe).
+Module Type HasT.
+  Parameter t : Type.
+End HasT.
+
+Module Type ArrayListOps (Idx : HasT).
 
   Parameter array : Type -> Type.
 
@@ -27,31 +31,46 @@ Module Type ArrayListOps (Idx : EqLtLe).
    *)
   Parameter set : forall {A}, array A -> Idx.t -> A -> array A.
 
- 
-  (*TODO: how best to handle optional max?
-    make extend op. return an option?
-    shouldn't extend be wrapped into set?
-  Parameter set_extensible : forall {A}, array A -> Idx.t -> A -> array A.
-   *)
-
   Parameter length : forall {A}, array A -> Idx.t.
-
-  (* TODO: length is broken in impl below; fix and then restore this
-  (* Note: returns l if (length l) = max_length *)
-  Definition cons {A} a (l : array A) : array A :=
-    set l (length l) a.
-   *)
-
-  (*If this is none, no max length*)
-  Parameter max_length : option Idx.t.
+  
+  Parameter alloc : forall {A}, array A -> A -> Idx.t * array A.
 
 End ArrayListOps.
 
+Module Type NatLike (Idx : EqLtLe).
+
+  Include OrderFunctions Idx.
+
+  Parameter zero : Idx.t.
+  
+  Parameter succ : Idx.t -> Idx.t.
+
+  Parameter isTop : Idx.t -> bool.
+
+  Axiom zero_spec
+    : forall a, Idx.le zero a.
+
+  Axiom succ_greater
+    : forall a,
+      (exists b, Idx.lt a b) ->
+      Idx.lt a (succ a).
+  
+  Axiom succ_least
+    : forall a b,
+      Idx.lt a b ->
+      Idx.le (succ a) b.
+
+  Axiom isTop_spec
+    : forall a,
+      isTop a = false
+      <-> (exists b, Idx.lt a b).
+
+End NatLike.
 
 (*Copied and modified from primitive arrays*)
 Module ArrayNotations
        (Idx : EqLtLe)
-       (Import IdxFns : OrderFunctions Idx)
+       (Import IdxFns : NatLike Idx)
        (Import AO : (ArrayListOps Idx)).
   Delimit Scope array_scope with array.
   Notation "t .[ i ]" :=
@@ -60,45 +79,51 @@ Module ArrayNotations
   Notation "t .[ i <- a ]" :=
     (set t i a)
       (at level 2, left associativity, format "t .[ i <- a ]").
-  Notation "a ::! t" :=
-    (cons a t)
-      (at level 60, right associativity, format "a ::! t").
+  Notation "'new!' a :: t" :=
+    (alloc t a)
+      (at level 60, right associativity, format "new! a :: t").
   
   Infix "=?" := eqb (at level 70, no associativity).
   Infix "<?" := ltb (at level 70, no associativity).
   Infix "<=?" := leb (at level 70, no associativity).
+  Notation "i .+1" := (succ i) (at level 70, no associativity).
 End ArrayNotations.
 
 Module Type ArrayListSpec 
        (Idx : EqLtLe)
-       (Import IdxFns : OrderFunctions Idx)
+       (Import IdxFns : NatLike Idx)
        (Import AO : (ArrayListOps Idx)).
 
   Module Import N := (ArrayNotations Idx IdxFns AO).
 
-  (* Checks whether an index is writable
-     i.e. whether it's less than the maximum size of an array
-   *)
-  Definition in_bounds i :=
-    match max_length with
-    | Some m => i <? m
-    | None => true
-    end.
-  
-  Axiom get_set_same : forall A t i (a:A), in_bounds i = true ->t.[i<-a].[i] = a.
+  Axiom get_set_same : forall A t i (a:A), t.[i<-a].[i] = a.
   Axiom get_set_other : forall A t i j (a:A), i <> j -> t.[i<-a].[j] = t.[j].
-
   
   Axiom get_make : forall A (a:A) i, (make a).[i] = a.
 
+  Axiom get_alloc_same
+    : forall A l (a:A) l' i,
+      (i,l') = alloc l a ->
+      l'.[i] = a.
+
+  Axiom alloc_fresh
+    : forall A l (a:A) l' i,
+      (i,l') = alloc l a ->
+      (exists i', Idx.lt (length l) i') ->
+      Idx.lt (length l) i.
+
+  (*TODO: move to the right place*)
   Definition max (x y : Idx.t) :=
     if x <=? y then y else x.
-    
-  (* Note: differs from PArray because set dynamically scales *)
-  Axiom length_set : forall A t i (a:A),
-      length t.[i<-a] = if in_bounds i then max (length t) i else (length t).
+
+  Axiom length_set :
+    forall A t i (a : A),
+      length t.[i <- a] = max (length t) (i.+1).
+
+  Axiom length_make : forall A (a:A), length (make a) = zero.
 
   (*TODO: rest of array axioms as necessary *)
+  
 End ArrayListSpec.  
 
 Module Int63EqLtLe <: EqLtLe.
@@ -111,7 +136,24 @@ Module Int63EqLtLe <: EqLtLe.
 
 End Int63EqLtLe.
 
-Module Int63Fns <: OrderFunctions Int63EqLtLe.
+
+
+Import Int63 Lia.
+
+Lemma max_int_greatest
+  : forall a, Int63EqLtLe.le a max_int.
+Proof.
+  unfold Int63EqLtLe.le.
+  intro a.
+  let x := eval vm_compute in  φ (max_int)%int63 in 
+      change ( φ (max_int)%int63) with x.
+  pose proof (to_Z_bounded a).
+  let x := eval vm_compute in  wB in 
+      change wB with x in H.
+  lia.
+Qed.
+
+Module Int63Fns <: NatLike Int63EqLtLe.
 
   Import Int63 Int63EqLtLe.
   Definition compare := compare.
@@ -132,6 +174,120 @@ Module Int63Fns <: OrderFunctions Int63EqLtLe.
   Definition eqb_eq : forall x y : int, eqb x y = true <-> eq x y := eqb_spec.
   Definition ltb_lt : forall x y : int, ltb x y = true <-> lt x y := ltb_spec.
   Definition leb_le : forall x y : int, leb x y = true <-> le x y := leb_spec.
+
+  Definition zero : int := 0.
+
+  Definition succ : int -> int := succ.
+
+  Definition isTop i :=
+    eqb i max_int.
+
+  Lemma zero_spec : forall i, le zero i.
+  Proof.
+    apply to_Z_bounded.
+  Qed.
+
+  Lemma eq_max_int_no_greater
+    : forall a,
+      a <> max_int
+      <-> (exists b, lt a b).
+  Proof.
+    split; intros.
+    {
+      exists max_int.
+      unfold lt.
+      pose proof (fun p => H (to_Z_inj _ _ p)).
+      change (?a -> False) with (not a) in H0.
+      pose proof (max_int_greatest a).
+      unfold le in*.
+      lia.
+    }
+    {
+      unfold lt in *.
+      firstorder.
+      intro.
+      subst.
+      pose proof (max_int_greatest x).
+      unfold le in *.
+      lia.
+    }
+  Qed.
+  
+  Lemma neq_max_int_lt
+    : forall a,
+      a <> max_int
+      <-> lt a max_int.
+  Proof.
+    intro a.
+    rewrite eq_max_int_no_greater.
+    unfold lt; split; [ intros [b H] | exists max_int; auto].
+    pose proof (max_int_greatest b).
+    unfold le in *.
+    lia.
+  Qed. 
+
+  Lemma isTop_spec
+    : forall a,
+      isTop a = false
+      <-> (exists b, lt a b).
+  Proof.
+    intro a.
+    rewrite <- eq_max_int_no_greater.
+    remember (isTop a) as b.
+    unfold isTop in *.
+    destruct b; split; try intuition congruence.
+    {
+      symmetry in Heqb.
+      rewrite eqb_eq in Heqb.
+      unfold eq in *.
+      subst.
+      tauto.
+    }
+    {
+      intros _.
+      intro Heq; rewrite <- eqb_eq in Heq.
+      rewrite Heq in Heqb.
+      inversion Heqb.
+    }
+  Qed.
+  
+  Lemma succ_greater
+    : forall a,
+      (exists b, lt a b) ->
+      lt a (succ a).
+  Proof.
+    intro a.
+    rewrite <- eq_max_int_no_greater.
+    rewrite neq_max_int_lt.
+    unfold lt.
+    rewrite succ_spec.
+    intros.
+    rewrite Z.mod_small.
+    lia.
+    let x := eval vm_compute in  φ (max_int)%int63 in 
+        change ( φ (max_int)%int63) with x in H.
+    pose proof (to_Z_bounded a).
+    let x := eval vm_compute in  wB in 
+        change wB with x.
+    lia.
+  Qed.
+  
+  Lemma succ_least
+    : forall a b,
+      lt a b ->
+      le (succ a) b.
+  Proof.
+    unfold lt.
+    unfold le.
+    unfold succ.
+    unfold Int63.succ.
+    intros.
+    rewrite add_spec.
+    pose proof (to_Z_bounded a).
+    rewrite to_Z_1.
+    pose proof (Z.mod_le (φ (a)%int63 + 1) wB ltac:(lia) wB_pos).
+    lia.
+  Qed.
 
 End Int63Fns.
 
@@ -156,23 +312,36 @@ Definition intrec {A} base rec i : A :=
   posZrec base rec' (to_Z i).
 
 
+Import Int63 PArray.
+
+Compute max_length.
+Compute max_int.
+Compute (max_int/max_length)%int63.
+
 Module PArrayListOps <: (ArrayListOps Int63EqLtLe).
 
   Import Int63 PArray.
   
-  Definition array := array.
+  Record array_rec (A : Type) :=
+    MkArr {
+        arr : PArray.array A;
+        len : int
+      }.
+  Definition array := array_rec.
+  Arguments MkArr {_}.
+  Arguments arr {_}.
+  Arguments len {_}.
 
   (* initial size is hardcoded *)
-  Definition make {A} := @make A (4)%int63.
+  Definition make {A} default := MkArr (@make A (4)%int63 default) 0.
 
-  Definition get {A} := @get A.
+  Definition get {A} l := @get A l.(arr).
 
-
-  Definition copyNth {A} l i (l' : array A) : array A :=
+  Definition copyNth {A} l i (l' : PArray.array A) : PArray.array A :=
     l'.[i <- l.[i]].
   
   (* TODO: this one is tricky. Make sure it computes nicely *)
-  Definition copyUpTo {A} (l l' : array A) : int -> array A :=
+  Definition copyUpTo {A} (l l' : PArray.array A) : int -> PArray.array A :=
     intrec l (copyNth l').
 
   (*TODO: duplicated; refactor*)
@@ -180,26 +349,22 @@ Module PArrayListOps <: (ArrayListOps Int63EqLtLe).
     if leb x y then y else x.
 
   (*TODO: separate order notations so that I can use them here*)
-  Definition expandToContain {A} i (l : array A) :=
-    let len := length l in
-    if ltb i len then l
+  Definition expandToContain {A} i '(MkArr l len_l) : array A :=
+    let backed_len := length l in
+    if ltb i backed_len then MkArr l (max i len_l)
     else
-      let len' := max (2 * len)%int63 i in
-      copyUpTo l (PArray.make len (get l len)) len.
+      let backed_len' := max (2 * backed_len)%int63 i in
+      let default := PArray.get l backed_len in
+      MkArr (copyUpTo (PArray.make backed_len' default) l len_l) i.    
   
   (* Dynamically grows the array as necessary *)
-  Definition set {A} l i (a : A) := set (expandToContain i l) i a.      
- 
-  Definition length {A} := @length A.
+  Definition set {A} l i (a : A) :=
+    let '(MkArr l len_l) := (expandToContain (i+1) l) in
+    MkArr (set l i a) len_l.
 
-  (* TODO: does not work due to exponential growth in copy.
-     Will need to keep a counter w/ filled length to make this work
-  (* Note: returns l if (length l) = max_length *)
-  Definition cons {A} a (l : array A) : array A :=
-    set l (length l) a.
-   *)
-
-  Definition max_length := Some max_length.
+  Definition length := @len.
+  
+  Definition alloc {A} l (a : A) := (l.(len),set l l.(len) a).
 
 End PArrayListOps.
 
@@ -208,7 +373,16 @@ Import PArrayListOps.
 Module Import N := (ArrayNotations Int63EqLtLe Int63Fns PArrayListOps).
 
 Compute make 4.
-Compute (expandToContain 5 (make 4)).
+Time Compute
+  let '(_,l) := (alloc (make 3) 2) in
+  let '(_,l) := (alloc l 2) in
+  let '(_,l) := (alloc l 2) in
+  let '(_,l) := (alloc l 2) in
+  let '(_,l) := (alloc l 2) in
+  l.
+Time Compute (expandToContain 2 (make 4)).[6555 <- 5]%int63.
+
+
 Compute (make 4).[5 <- 5]%int63.
 (*TODO: needs to be instant*)
 Compute (make 4).[33 <- 5]%int63.
